Learn.LowStar.Queue.Impl.fst
@@ -2,6 +2,7 @@ module Learn.LowStar.Queue.Impl
 
 module U   = Learn.Util
 module L   = FStar.List.Pure
+module Ll  = Learn.List
 module B   = LowStar.Buffer
 module M   = LowStar.Modifies
 module G   = FStar.Ghost
@@ -13,179 +14,181 @@ module LLoops = Learn.LowStar.Loops
 open LowStar.BufferOps
 open FStar.HyperStack.ST
 
-open Learn.LowStar.Queue.Data
+open Learn.LowStar.Queue.Param
 open Learn.LowStar.Queue.Prop
 
 #set-options "--fuel 2 --ifuel 0"
 
 (* [malloc] *)
 
-let malloc (a : Type) (r : HS.rid)
-  : ST (queue a)
+inline_for_extraction
+let malloc (#c : Type) (a : queue_param c) (r : HS.rid)
+  : ST (queue c)
        (requires fun _       -> ST.is_eternal_region r)
        (ensures  fun h0 q h1 -> M.(modifies loc_none h0 h1 /\
-                                fresh_loc (loc_buffer q) h0 h1 /\
-                                loc_includes (loc_region_only true r) (loc_buffer q) /\
+                                fresh_loc (loc_addr_of_buffer q) h0 h1 /\
+                                loc_includes (loc_region_only true r) (loc_addr_of_buffer q) /\
                                 freeable q) /\
-                             live_queue h1 q [])
+                             live_queue a h1 q [])
   =
-    B.malloc #(queue_st a) r ({q_exit = B.null; q_entry = B.null}) 1ul
+    B.malloc #(queue_st c) r ({q_exit = B.null; q_entry = B.null}) 1ul
 
 (* [free] *)
 
-let free (#a : Type) (q : queue a)
+inline_for_extraction
+let free (#c : Type) (a : queue_param c) (q : queue c)
   : ST  unit
-       (requires fun h      -> live_queue h q [] /\ M.freeable q)
+       (requires fun h      -> live_queue a h q [] /\ M.freeable q)
        (ensures  fun h b h' -> M.(modifies (loc_addr_of_buffer q) h h'))
   =
     B.free q
 
 (* [is_empty] *)
 
-let is_empty (#a : Type) (x : B.pointer (cell a)) (q : queue a) (l : G.erased (cell_list a))
+inline_for_extraction
+let is_empty (#c : Type) (a : queue_param c) (q : queue c) (l : G.erased (cell_list c))
   : Stack  bool
-          (requires fun h      -> live_queue h q l)
+          (requires fun h      -> live_queue a h q l)
           (ensures  fun h b h' -> h' == h /\ b = Nil? l)
-  = B.is_null (sgn_entry (q.(0ul)).q_exit (sg_of_cells l))
+  = B.is_null (sgn_entry a (q.(0ul)).q_exit (sg_of_cells l))
 
 (* [enqueue] *)
 
-let enqueue (#a : Type) (x : B.pointer (cell a)) (q : queue a) (l : G.erased (cell_list a))
+inline_for_extraction
+let enqueue (#c : Type) (a : queue_param c)
+  (get_next : U.alias a.get_next) (set_next : U.alias a.set_next)
+  (x : B.pointer c) (q : queue c) (l : G.erased (cell_list c))
   : Stack  unit
-          (requires fun h0       -> wf_queue q l /\ live_queue h0 q l /\
+          (requires fun h0       -> wf_queue q l /\ live_queue a h0 q l /\
                                  B.live h0 x /\
                                  M.(loc_disjoint (loc_buffer x) (loc_queue q l)))
           (ensures  fun h0 () h1 -> M.(modifies (loc_union (loc_buffer x) (loc_queue q l)) h0 h1) /\
-                                 mod_next h0 h1 x /\ mod_next_list h0 h1 l /\
-                                 live_queue h1 q (L.snoc (G.reveal l,x)))
+                                 mod_next a h0 h1 x /\ mod_next_list a h0 h1 l /\
+                                 live_queue a h1 q (L.snoc (G.reveal l,x)))
   =   
+      open_queue_param a;
       let h0 = ST.get () in
       let sg = G.hide (sg_of_cells l) in
-    x.(0ul) <- {x.(0ul) with next = B.null};
-    if B.is_null (sg_last (q.(0ul)).q_entry sg) then begin
+    x.(0ul) <- set_next (x.(0ul)) B.null;
+    if B.is_null (sg_last a (q.(0ul)).q_entry sg) then begin
       q.(0ul) <- {q_exit = x; q_entry = x};
-        let _ = sg_mksglt x B.null in ()
+        let _ = sg_mksglt a x B.null in ()
     end else begin
         let ini = G.hide (unsnoc_seg sg)._1 in
         let tls = G.hide (unsnoc_seg sg)._2 in
-        sg_unapp ini tls;
-        let tl = (sg_uncons tls)._1 in
+        sg_unapp a ini tls;
+        let tl = (sg_uncons a tls)._1 in
         assert (loc_seg tls.segment == B.loc_buffer tl);
         assert (loc_seg sg.segment  == M.(loc_union (loc_seg ini.segment) (B.loc_buffer tl)));
-      (q.(0ul)).q_entry.(0ul) <- {(q.(0ul)).q_entry.(0ul) with next = x};
+      (q.(0ul)).q_entry.(0ul) <- set_next (q.(0ul)).q_entry.(0ul) x;
       q.(0ul) <- {q.(0ul) with q_entry = x};
         let h1 = ST.get () in
-        let sg' = sg_mkapp ini (sg_mkcons tl (sg_mksglt x B.null)) in
+        let sg' = sg_mkapp a ini (sg_mkcons a tl (sg_mksglt a x B.null)) in
         L.append_assoc (ini.segment) [G.reveal tl] [x];
         assert (L.snoc (G.reveal l,x) == sg'.segment);
         append_last_cell sg.segment [x];
         assert (sg_entry sg' == sg_entry sg);
-        U.assert_by (mod_next_list h0 h1 l) (fun () ->
-          append_seg_live h0 ini tls;
-          sg_uncons_lem h0 tls;
+        U.assert_by (mod_next_list a h0 h1 l) (fun () ->
+          append_seg_live a h0 ini tls;
+          sg_uncons_lem a h0 tls;
           let md = M.(loc_union (loc_buffer x) (loc_union (loc_buffer tl) (loc_buffer q))) in
-          disjoint_mod_next_seg h0 h1 md ini;
-          assert (mod_next_list h0 h1 [G.reveal tl]))
+          disjoint_mod_next_seg a h0 h1 md ini;
+          assert (mod_next_list a h0 h1 [G.reveal tl]))
     end
 
 (* [dequeue] *)
 
-let dequeue (#a : Type) (q : queue a) (l : G.erased (cell_list a))
-  : Stack (B.pointer (cell a))
-          (requires fun h0       -> wf_queue q l /\ live_queue h0 q l /\
+inline_for_extraction
+let dequeue (#c : Type) (a : queue_param c) (get_next : U.alias a.get_next)
+            (q : queue c) (l : G.erased (cell_list c))
+  : Stack (B.pointer c)
+          (requires fun h0       -> wf_queue q l /\ live_queue a h0 q l /\
                                  Cons? l)
           (ensures  fun h0 rt h1 -> M.modifies (loc_queue q l) h0 h1 /\
-                                 mod_next_list h0 h1 l /\
+                                 mod_next_list a h0 h1 l /\
                                  rt == L.hd l /\
-                                 live_queue h1 q (L.tl l) /\ B.live h1 rt)
+                                 live_queue a h1 q (L.tl l) /\ B.live h1 rt)
   =
+      open_queue_param a;
       let h0 = ST.get () in
       let sg = G.hide (sg_of_cells l) in
-      let hd,sg' = sg_uncons sg in
+      let hd,sg' = sg_uncons a sg in
     let rt = (q.(0ul)).q_exit in
-    q.(0ul) <- { q.(0ul) with q_exit = sg_next rt sg };
-    if B.is_null (sgn_entry (q.(0ul)).q_exit (G.reveal sg')) then
+    q.(0ul) <- { q.(0ul) with q_exit = sg_next a get_next rt sg };
+    if B.is_null (sgn_entry a (q.(0ul)).q_exit (G.reveal sg')) then
       q.(0ul) <- { q.(0ul) with q_entry = B.null };
       let h1 = ST.get () in G.hide(
       let md = M.(loc_union (loc_buffer hd) (loc_buffer q)) in
-      disjoint_mod_next_seg h0 h1 md sg');
+      disjoint_mod_next_seg a h0 h1 md sg');
     rt
 
 (* [find] *)
 
-#push-options "--ifuel 1"
-let rec find_gtot (#a:Type) (f:a -> GTot bool) (l:list a) : GTot (option (x:a{f x})) (decreases l)
-  = match l with
-  | [] -> None
-  | hd :: tl -> if f hd then Some #(x:a{f x}) hd else find_gtot f tl
-#pop-options
-
-
 inline_for_extraction
-let rec list_find_rec (#a : Type)
-         (p : cell_ptr a) (sg : G.erased (list_nil a))
+let rec list_find_rec (#c : Type) (a : queue_param c) (get_next : U.alias a.get_next)
+         (p : cell_ptr c) (sg : G.erased (list_nil c))
          (h0 : HS.mem) (* needed to specify [f] *)
-         (spec_f : (x : B.pointer (cell a) -> GTot bool))
-         (f : (x : B.pointer (cell a)) ->
+         (spec_f : (x : B.pointer c -> GTot bool))
+         (f : (x : B.pointer c) ->
               Stack bool
                     (requires fun h      -> h == h0 /\ B.live h x /\ L.memP x sg.segment)
                     (ensures  fun h b h' -> h' == h /\ b = spec_f x))
-   : Stack (B.pointer_or_null (cell a))
-          (requires fun h       -> h == h0 /\ live_seg h sg /\ p == sg_entry sg)
+   : Stack (cell_ptr c)
+          (requires fun h       -> h == h0 /\ live_seg a h sg /\ p == sg_entry sg)
           (ensures  fun h rt h' -> h' == h /\
-                                rt == (match find_gtot spec_f sg.segment with
+                                rt == (match Ll.find_gtot spec_f sg.segment with
                                        | Some p -> p | None -> B.null))
    =
-     if B.is_null (sgn_entry p sg) then B.null
+     if B.is_null (sgn_entry a p sg) then B.null
      else begin
-         let tl = (sg_uncons (G.reveal sg))._2 in
+         let tl = (sg_uncons a (G.reveal sg))._2 in
        if f p then p
-       else list_find_rec (sg_next p (G.reveal sg)) (G.reveal tl) h0 spec_f f
+       else list_find_rec a get_next (sg_next a get_next p (G.reveal sg)) (G.reveal tl) h0 spec_f f
      end
 
 #push-options "--z3rlimit 20"
 inline_for_extraction
-let list_find_loop (#a : Type)
-         (p : cell_ptr a) (sg0 : G.erased (list_nil a))
+let list_find_loop (#c : Type) (a : queue_param c) (get_next : U.alias a.get_next)
+         (p : cell_ptr c) (sg0 : G.erased (list_nil c))
          (h0  : HS.mem)
-         (spec_f : (x : B.pointer (cell a) -> GTot bool))
-         (f : (x : B.pointer (cell a)) ->
+         (spec_f : (x : B.pointer c -> GTot bool))
+         (f : (x : B.pointer c) ->
               Stack bool
                     (requires fun h -> M.(modifies loc_none h0 h) /\ B.live h x /\ L.memP x sg0.segment)
                     (ensures  fun h b h' -> M.(modifies loc_none h h') /\ b = spec_f x))
-   : Stack (B.pointer_or_null (cell a))
-          (requires fun h       -> h == h0 /\ live_seg h sg0 /\ p == sg_entry sg0)
+   : Stack (cell_ptr c)
+          (requires fun h       -> h == h0 /\ live_seg a h sg0 /\ p == sg_entry sg0)
           (ensures  fun h rt h' -> M.(modifies loc_none h h') /\
-                                rt == (match find_gtot spec_f sg0.segment with
+                                rt == (match Ll.find_gtot spec_f sg0.segment with
                                        | Some p -> p | None -> B.null))
    =
      push_frame ();
        let h0' = ST.get () in
-     let it = B.alloca #(cell_ptr a & G.erased (list_nil a)) (p, sg0) 1ul in
-     let rt = B.alloca #(cell_ptr a) B.null 1ul in
+     let it = B.alloca #(cell_ptr c & G.erased (list_nil c)) (p, sg0) 1ul in
+     let rt = B.alloca #(cell_ptr c) B.null 1ul in
        let lloc = G.hide (M.(loc_union (loc_buffer it) (loc_buffer rt))) in
      let pre h1 : prop =
          M.(let (p, sg) = deref h1 it in
          modifies loc_none h0 h1 /\
          live h1 it /\ live h1 rt /\
-         live_seg h1 (deref h1 it)._2 /\
+         live_seg a h1 (deref h1 it)._2 /\
          loc_disjoint (loc_buffer it) (loc_seg sg.segment) /\
          p == sg_entry sg /\
          (forall x . {:pattern (L.memP x sg0.segment)} L.memP x sg.segment ==> L.memP x sg0.segment))
      in let post_test h1 (b:bool) : prop =
          (Cons? (B.deref h1 it)._2.segment <==> b)
-     in let post h1 (x : cell_ptr a) h2 : prop =
+     in let post h1 (x : cell_ptr c) h2 : prop =
          let _,sg = B.deref h1 it in
          let dflt = B.deref h1 rt in
          M.(modifies lloc h1 h2) /\
-         x == (match find_gtot spec_f sg.segment with
+         x == (match Ll.find_gtot spec_f sg.segment with
                      | Some p -> p | None -> dflt)
      in
      let test () : Stack bool
               (requires fun h1       -> pre h1)
               (ensures  fun h1 b h1' -> h1' == h1 /\ post_test h1 b)
        =   let sg = (it.(0ul))._2 in
-         not (B.is_null (sgn_entry (it.(0ul))._1 sg))
+         not (B.is_null (sgn_entry a (it.(0ul))._1 sg))
      in
      let body () : Stack unit
               (requires fun h1       -> pre h1 /\ Cons? (B.deref h1 it)._2.segment)
@@ -193,13 +196,13 @@ let list_find_loop (#a : Type)
                                      LLoops.tail_rec_post h2 (post h2) (post h1))
        =   let h1 = ST.get () in
            let sg = (it.(0ul))._2 in
-           let tl = (sg_uncons (G.reveal sg))._2 in
-         if f (sgn_entry (it.(0ul))._1 sg)
+           let tl = (sg_uncons a (G.reveal sg))._2 in
+         if f (sgn_entry a (it.(0ul))._1 sg)
          then begin
            rt.(0ul) <- (it.(0ul))._1;
-           it.(0ul) <- (B.null, G.hide (empty_list a))
+           it.(0ul) <- (B.null, G.hide (empty_list c))
          end else begin
-           it.(0ul) <- (sg_next (it.(0ul))._1 (G.hide (G.reveal sg)), (G.hide (G.reveal tl)))
+           it.(0ul) <- (sg_next a get_next (it.(0ul))._1 (G.hide (G.reveal sg)), (G.hide (G.reveal tl)))
          end;
            let h2 = ST.get () in
            assert M.(modifies lloc h0 h2);
@@ -212,70 +215,18 @@ let list_find_loop (#a : Type)
      rt_v
 #pop-options
 
-
 inline_for_extraction
-let find (#a : Type)
-         (q : queue a) (l : G.erased (cell_list a))
+let find (#c : Type) (a : queue_param c) (get_next : U.alias a.get_next)
+         (q : queue c) (l : G.erased (cell_list c))
          (h0  : HS.mem)
-         (spec_f : (x : B.pointer (cell a) -> GTot bool))
-         (f : (x : B.pointer (cell a)) ->
+         (spec_f : (x : B.pointer c -> GTot bool))
+         (f : (x : B.pointer c) ->
               Stack bool
                     (requires fun h -> M.(modifies loc_none h0 h) /\ B.live h x /\ L.memP x l)
                     (ensures  fun h b h' -> M.(modifies loc_none h h') /\ b = spec_f x))
-  : Stack (B.pointer_or_null (cell a))
-          (requires fun h       -> h == h0 /\ live_queue h q l)
+  : Stack (cell_ptr c)
+          (requires fun h       -> h == h0 /\ live_queue a h q l)
           (ensures  fun h rt h' -> M.(modifies loc_none h h') /\
-                                rt == (match find_gtot spec_f l with
+                                rt == (match Ll.find_gtot spec_f l with
                                        | Some p -> p | None -> B.null))
-  = list_find_loop ((q.(0ul)).q_exit) (sg_of_cells l) h0 spec_f f
- 
-(* ---------- *)
-
-let malloc_u32   = malloc    U32.t
-let is_empty_u32 = is_empty #U32.t
-let enqueue_u32  = enqueue  #U32.t
-let dequeue_u32  = dequeue  #U32.t
-
-let mem_42 (q : queue U32.t) (l : G.erased (cell_list U32.t))
-  : Stack (B.pointer_or_null (cell U32.t))
-          (requires fun h       -> live_queue h q l)
-          (ensures  fun h rt h' -> M.(modifies loc_none h h') /\
-                    rt == (match find_gtot (fun (c:B.pointer (cell U32.t)) -> (B.deref h c).data = 42ul) l with
-                           | Some p -> p | None -> B.null))
-  =   let h = ST.get () in
-    find q l h (fun c -> (B.deref h c).data = 42ul)
-               (fun c -> live_seg_cell h (sg_of_cells l) c; (c.(0ul)).data = 42ul)
-
-#push-options "--fuel 3 --z3rlimit 40"
-let test_queue_spec () : St unit
-  =
-    push_frame ();
-    let q = malloc U32.t HS.root in
-    let x0 = B.malloc #(cell U32.t) HS.root ({data = 5ul; next = B.null}) 1ul in
-    enqueue x0 q [];
-      (let h = ST.get () in assert (live_queue h q [x0]));
-      (let d = (x0.(0ul)).data in assert (d == 5ul));
-      (let f = mem_42 q [x0] in assert (f == B.null));
-      (let h0 = ST.get () in
-    x0.(0ul) <- {x0.(0ul) with data = 42ul};
-      (let h1 = ST.get () in
-       frame_seg_mod_data h0 h1 (sg_of_cells [x0]);
-       assert (live_queue h1 q [x0])));
-      (let f = mem_42 q [x0] in assert (f == x0));
-
-    let x12 = B.alloca #(cell U32.t) ({data = 7ul; next = B.null}) 2ul in
-    let x1 = B.sub x12 0ul 1ul in let x2 = B.sub x12 1ul 1ul in
-    enqueue x1 q [x0];
-      (let h0 = ST.get () in assert (live_queue h0 q [x0; x1]);
-    x2.(0ul) <- {x2.(0ul) with data = 8ul};
-      let h1 = ST.get () in
-      frame_seg h0 h1 (sg_of_cells [x0; x1]) (M.loc_buffer x2);
-      assert (live_queue h1 q [x0; x1]));
-    let x0' = dequeue q [x0; x1] in
-      assert (x0' == x0);
-    B.free x0;
-    let x1' = dequeue q [x1] in
-      (assert (x1' == x1); let d = (x1.(0ul)).data in assert (d = 7ul));
-    pop_frame ();
-    free q
-#pop-options
+  = list_find_loop a get_next ((q.(0ul)).q_exit) (sg_of_cells l) h0 spec_f f
