Learn.LowStar.Queue.Prop.fst
@@ -1,61 +1,71 @@
 module Learn.LowStar.Queue.Prop
 
+module M   = LowStar.Modifies
+
 let live_seg = live_seg_def
 
-let live_seg_unfold a = assert_norm (live_seg #a == live_seg_def #a)
+let live_seg_unfold #c a = assert_norm (live_seg a == live_seg_def a)
 
-let rec loc_seg_live_in #a h sg =
+let rec loc_seg_live_in #c a h sg =
   match sg.segment with
   | []    -> ()
-  | _ :: _ -> loc_seg_live_in h (tail_seg sg)
+  | _ :: _ -> loc_seg_live_in a h (tail_seg sg)
 
-let rec live_seg_cell #a h sg c =
+let rec loc_seg_cell #c sg x =
+  match sg with
+  | [] -> ()
+  | hd :: tl -> eliminate x == hd \/ L.memP x tl
+                returns M.(loc_seg sg `loc_includes` loc_buffer x)
+                   with pf_hd. ()
+                    and pf_tl. loc_seg_cell tl x
+
+let rec live_seg_cell #c a h sg x =
   match sg.segment with
   | [] -> ()
-  | hd :: tl -> eliminate c == hd \/ L.memP c tl
-                returns B.live h c
+  | hd :: tl -> eliminate x == hd \/ L.memP x tl
+                returns B.live h x
                    with pf_hd. ()
-                    and pf_tl. live_seg_cell h (tail_seg sg) c
+                    and pf_tl. live_seg_cell a h (tail_seg sg) x
 
-let rec frame_seg #a h0 h1 sg r =
+let rec frame_seg #c a h0 h1 sg r =
   match sg.segment with
   | []    -> ()
-  | _ :: _ -> frame_seg h0 h1 (tail_seg sg) r
+  | _ :: _ -> frame_seg a h0 h1 (tail_seg sg) r
 
-let rec frame_seg_mod_data #a h0 h1 sg =
+let rec frame_seg_mod_data #c a h0 h1 sg =
   match sg.segment with
   | []    -> ()
-  | _ :: _ -> frame_seg_mod_data h0 h1 (tail_seg sg)
+  | _ :: _ -> frame_seg_mod_data a h0 h1 (tail_seg sg)
 
-let rec disjoint_mod_next_seg #a h0 h1 p sg
+let rec disjoint_mod_next_seg #c a h0 h1 p sg
   = match sg.segment with
     | [] -> ()
-    | _ :: _ -> disjoint_mod_next_seg h0 h1 p (tail_seg sg)
+    | _ :: _ -> disjoint_mod_next_seg a h0 h1 p (tail_seg sg)
 
-let rec append_seg_live #a h sg0 sg1 =
+let rec append_seg_live #c a h sg0 sg1 =
   match sg0.segment with
   | [] -> ()
-  | _ :: _ -> append_seg_live h (tail_seg sg0) sg1
+  | _ :: _ -> append_seg_live a h (tail_seg sg0) sg1
 
-let rec last_cell_live #a h sg =
+let rec last_cell_live #c a h sg =
   match sg.segment with
   | []  -> ()
   | [_] -> ()
-  | _ :: _ -> last_cell_live h (tail_seg sg)
+  | _ :: _ -> last_cell_live a h (tail_seg sg)
 
-let empty_live #a exit h = ()
+let empty_live #c a exit h = ()
 
-let sg_mkcons_lem #a h hd tl = ()
+let sg_mkcons_lem #c a h hd tl = ()
 
-let sg_uncons_lem #a h sg = ()
+let sg_uncons_lem #c a h sg = ()
 
-let entry_null_is_empty #a h sg =
+let entry_null_is_empty #c a h sg =
   B.null_unique (sg_entry sg)
 
-let list_nil_entry_nnull #a h sg = ()
+let list_nil_entry_nnull #c a h sg = ()
 
 inline_for_extraction
-let sgn_entry #a p sg = p
+let sgn_entry #c a p sg = p
 
 inline_for_extraction
-let sg_next #a p sg = (p.(0ul)).next
+let sg_next #c a get_next p sg = get_next (p.(0ul))
