Learn.LowStar.Queue.Prop.fsti
@@ -1,5 +1,6 @@
 module Learn.LowStar.Queue.Prop
 
+module U   = Learn.Util
 module L   = FStar.List.Pure
 module Ll  = Learn.List
 module B   = LowStar.Buffer
@@ -11,50 +12,57 @@ module ST  = FStar.HyperStack.ST
 open LowStar.BufferOps
 open FStar.HyperStack.ST
 
-open Learn.LowStar.Queue.Data
+open Learn.LowStar.Queue.Param
 
 
-let g_cell_next (#a : Type) (h : HS.mem) (p : B.pointer (cell a)) : GTot (cell_ptr a)
-  = (B.deref h p).next
+noeq
+type queue_st (c : Type) = {
+  q_exit  : cell_ptr c;
+  q_entry : cell_ptr c;
+}
+
+type queue (c : Type) = B.pointer (queue_st c)
+
+let g_cell_next (#c : Type) (a : queue_param c) (h : HS.mem) (p : B.pointer c) : GTot (cell_ptr c)
+  = a.get_next (B.deref h p)
+
 
 (** Ghost representation of the structures *)
 
 noextract noeq
-type list_seg (a : Type) = {
-  segment : list (B.pointer (cell a));
-  exit    : cell_ptr a
+type list_seg (c : Type) = {
+  segment : list (B.pointer c);
+  exit    : cell_ptr c
 }
 
-let list_nil (a : Type) : Type = sg:list_seg a{sg.exit == B.null}
+let list_nil (c : Type) : Type = sg:list_seg c{sg.exit == B.null}
 
-type cell_list (a : Type) = list (B.pointer (cell a))
-
-let sg_of_cells (#a : Type) (l : cell_list a) : list_nil a
+let sg_of_cells (#c : Type) (l : cell_list c) : list_nil c
   = { segment = l; exit = B.null }
 
 
-let sg_entry (#a : Type) (sg : list_seg a) : Tot (cell_ptr a)
+let sg_entry (#c : Type) (sg : list_seg c) : Tot (cell_ptr c)
   = match sg.segment with
     | []    -> sg.exit
     | hd :: _ -> hd
 
-let cons_seg (#a : Type) (hd : B.pointer (cell a)) (sg : list_seg a) : list_seg a
+let cons_seg (#c : Type) (hd : B.pointer c) (sg : list_seg c) : list_seg c
   = { sg with segment = hd :: sg.segment }
 
-let tail_seg (#a : Type) (sg : list_seg a)
-  : Pure (list_seg a) (requires Cons? sg.segment) (ensures fun _ -> True)
+let tail_seg (#c : Type) (sg : list_seg c)
+  : Pure (list_seg c) (requires Cons? sg.segment) (ensures fun _ -> True)
   = {sg with segment = L.tail sg.segment}
 
-let append_seg (#a : Type) (sg0 sg1 : list_seg a) : Tot (list_seg a)
+let append_seg (#c : Type) (sg0 sg1 : list_seg c) : Tot (list_seg c)
   = { segment = L.(sg0.segment @ sg1.segment);
       exit    = sg1.exit }
 
-let append_seg_assoc (#a : Type) (sg0 sg1 sg2 : list_seg a)
+let append_seg_assoc (#c : Type) (sg0 sg1 sg2 : list_seg c)
   : Lemma (ensures append_seg sg0 (append_seg sg1 sg2) == append_seg (append_seg sg0 sg1) sg2)
   = L.append_assoc sg0.segment sg1.segment sg2.segment
 
-let rec last_cell (#a : Type) (sg : cell_list a)
-  : Pure (cell_ptr a)
+let rec last_cell (#c : Type) (sg : cell_list c)
+  : Pure (cell_ptr c)
          (requires True)
          (ensures fun lt -> B.g_is_null lt <==> Nil? sg)
          (decreases sg)
@@ -66,30 +74,30 @@ let rec last_cell (#a : Type) (sg : cell_list a)
 
 (** Predicates *)
 
-let rec loc_seg (#a : Type) (sg : cell_list a) : GTot M.loc
+let rec loc_seg (#c : Type) (sg : cell_list c) : GTot M.loc
   (decreases sg)
   = match sg with
     | [] -> M.loc_none
     | hd :: tl -> M.(loc_union (loc_buffer hd) (loc_seg tl))
 
-let rec wf_seg (#a : Type) (sg : list_seg a) : Tot prop
-  (decreases sg.segment)
-  = match sg.segment with
+let rec wf_seg (#c : Type) (sg : cell_list c) : Tot prop
+  (decreases sg)
+  = match sg with
     | [] -> True
     | hd :: tl -> (M.loc_disjoint (B.loc_buffer hd) (loc_seg tl))
-             /\ wf_seg (tail_seg sg)
+             /\ wf_seg tl
 
-let rec live_seg_def (#a : Type) (h : HS.mem) (sg : list_seg a) : Tot prop
+let rec live_seg_def (#c : Type) (a : queue_param c) (h : HS.mem) (sg : list_seg c) : Tot prop
   (decreases sg.segment)
   = match sg.segment with
     | [] -> True
     | hd :: _ -> let sg' = tail_seg sg in
-               B.live h hd /\ g_cell_next h hd == sg_entry sg' /\ live_seg_def h sg'
+               B.live h hd /\ g_cell_next a h hd == sg_entry sg' /\ live_seg_def a h sg'
 
 (* ALT? [@@"opaque_to_smt"] + reveal_opaque *)
-val live_seg (#a : Type) (h : HS.mem) (sg : list_seg a) : Tot prop
+val live_seg (#c : Type) (a : queue_param c) (h : HS.mem) (sg : list_seg c) : Tot prop
 
-val live_seg_unfold : a:Type -> Lemma (live_seg #a == live_seg_def #a)
+val live_seg_unfold : #c:Type -> (a : queue_param c) -> Lemma (live_seg a == live_seg_def a)
 
 
 /// A queue is a [queue_st] with a linked list of [cell].
@@ -98,69 +106,56 @@ val live_seg_unfold : a:Type -> Lemma (live_seg #a == live_seg_def #a)
 ///   - [q_entry] points to the last element of the list (or null if the queue is empty)
 ///     ALT? unspecified if the queue is empty
 
-let loc_queue (#a : Type) (q : queue a) (l : cell_list a) : GTot M.loc =
+let loc_queue (#c : Type) (q : queue c) (l : cell_list c) : GTot M.loc =
   M.(loc_union (loc_buffer q) (loc_seg l))
 
-let wf_queue (#a : Type) (q : queue a) (l : cell_list a) : Tot prop =
-  wf_seg (sg_of_cells l) /\ M.(loc_disjoint (loc_buffer q) (loc_seg l))
+let wf_queue (#c : Type) (q : queue c) (l : cell_list c) : Tot prop =
+  wf_seg l /\ M.(loc_disjoint (loc_buffer q) (loc_seg l))
 
-let live_queue (#a : Type) (h : HS.mem) (q : queue a) (l : cell_list a) : Tot prop =
-  B.live h q /\ live_seg h (sg_of_cells l) /\
+let live_queue (#c : Type) (a : queue_param c) (h : HS.mem) (q : queue c) (l : cell_list c) : Tot prop =
+  B.live h q /\ live_seg a h (sg_of_cells l) /\
  (let qs = B.deref h q in
   qs.q_exit  == sg_entry (sg_of_cells l) /\
   qs.q_entry == last_cell l)
 
-let mod_next (#a : Type) (h0 h1 : HS.mem) (c : B.pointer (cell a)) : GTot prop
-  = B.live h0 c /\ B.live h1 c /\ (B.deref h0 c).data == (B.deref h1 c).data
-
-let mod_next_list (#a : Type) (h0 h1 : HS.mem) (cs : cell_list a)
-  : GTot prop
-  = Ll.g_for_allP cs (mod_next #a h0 h1)
-
-let mod_data (#a : Type) (h0 h1 : HS.mem) (c : B.pointer (cell a)) : GTot prop
-  = B.live h0 c /\ B.live h1 c /\ (B.deref h0 c).next == (B.deref h1 c).next
-
-let mod_data_list (#a : Type) (h0 h1 : HS.mem) (cs : cell_list a)
-  : GTot prop
-  = Ll.g_for_allP cs (mod_data #a h0 h1)
 
 (** Lemmas about the predicates *)
 
-val loc_seg_live_in (#a : Type) (h : HS.mem) (sg : list_seg a)
-  : Lemma (requires live_seg h sg) (ensures B.loc_in (loc_seg sg.segment) h)
+val loc_seg_live_in (#c : Type) (a : queue_param c) (h : HS.mem) (sg : list_seg c)
+  : Lemma (requires live_seg a h sg) (ensures B.loc_in (loc_seg sg.segment) h)
           (decreases sg.segment)
-    [SMTPat (live_seg h sg)]
+    [SMTPat (live_seg a h sg)]
 
-val live_seg_cell (#a : Type) (h : HS.mem) (sg : list_seg a) (c : B.pointer (cell a))
-  : Lemma (requires  live_seg h sg /\ L.memP c sg.segment)
-          (ensures   B.live h c)
-          (decreases sg.segment)
+val loc_seg_cell (#c : Type) (sg : cell_list c) (x : B.pointer c)
+  : Lemma (requires  L.memP x sg)
+          (ensures   M.(loc_seg sg `loc_includes` loc_buffer x))
+          (decreases sg)
 
-val frame_seg (#a : Type) (h0 h1 : HS.mem) (sg : list_seg a) (r : B.loc)
-  : Lemma (requires live_seg h0 sg /\ M.(modifies r h0 h1 /\ loc_disjoint r (loc_seg sg.segment)))
-          (ensures  live_seg h1 sg)
-          (decreases sg.segment)
-    [SMTPat (live_seg #a h0 sg); SMTPat (M.modifies r h0 h1)]
-
-val frame_seg_mod_data (#a : Type) (h0 h1 : HS.mem) (sg : list_seg a)
-  : Lemma (requires live_seg h0 sg /\ mod_data_list h0 h1 sg.segment)
-          (ensures  live_seg h1 sg)
+val live_seg_cell (#c : Type) (a : queue_param c) (h : HS.mem) (sg : list_seg c) (x : B.pointer c)
+  : Lemma (requires  live_seg a h sg /\ L.memP x sg.segment)
+          (ensures   B.live h x)
           (decreases sg.segment)
 
-let disjoint_mod_next (#a : Type) (h0 h1 : HS.mem) (p : M.loc) (c : B.pointer (cell a))
-  : Lemma (requires M.(loc_disjoint (loc_buffer c) p /\ live h0 c /\ modifies p h0 h1))
-          (ensures  mod_next h0 h1 c)
-  = ()
+val frame_seg (#c : Type) (a : queue_param c) (h0 h1 : HS.mem) (sg : list_seg c) (r : B.loc)
+  : Lemma (requires live_seg a h0 sg /\ M.(modifies r h0 h1 /\ loc_disjoint r (loc_seg sg.segment)))
+          (ensures  live_seg a h1 sg)
+          (decreases sg.segment)
+    [SMTPat (live_seg a h0 sg); SMTPat (M.modifies r h0 h1)]
 
-val disjoint_mod_next_seg (#a : Type) (h0 h1 : HS.mem) (p : M.loc) (sg : list_seg a)
+val frame_seg_mod_data (#c : Type) (a : queue_param c) (h0 h1 : HS.mem) (sg : list_seg c)
+  : Lemma (requires live_seg a h0 sg /\ mod_data_list a h0 h1 sg.segment)
+          (ensures  live_seg a h1 sg)
+          (decreases sg.segment)
+
+val disjoint_mod_next_seg (#c : Type) (a : queue_param c) (h0 h1 : HS.mem) (p : M.loc) (sg : list_seg c)
   : Lemma (requires  M.(loc_disjoint (loc_seg sg.segment) p /\
-                        live_seg h0 sg /\ modifies p h0 h1))
-          (ensures   mod_next_list h0 h1 sg.segment)
+                        live_seg a h0 sg /\ modifies p h0 h1))
+          (ensures   mod_next_list a h0 h1 sg.segment)
           (decreases sg.segment)
 
 
 
-let rec append_seg_loc (#a : Type) (sg0 sg1 : cell_list a)
+let rec append_seg_loc (#c : Type) (sg0 sg1 : cell_list c)
   : Lemma (ensures loc_seg L.(sg0@sg1) == M.loc_union (loc_seg sg0) (loc_seg sg1))
           (decreases sg0)
           [SMTPat (loc_seg L.(sg0@sg1))]
@@ -170,143 +165,144 @@ let rec append_seg_loc (#a : Type) (sg0 sg1 : cell_list a)
       append_seg_loc tl sg1;
       M.loc_union_assoc (M.loc_buffer hd) (loc_seg tl) (loc_seg sg1)
 
-let rec append_seg_wf (#a : Type) (sg0 sg1 : list_seg a)
-  : Lemma (ensures wf_seg (append_seg sg0 sg1) <==>
-                   wf_seg sg0 /\ wf_seg sg1 /\ M.loc_disjoint (loc_seg sg0.segment) (loc_seg sg1.segment))
-          (decreases sg0.segment)
-          [SMTPat (wf_seg (append_seg sg0 sg1))]
-  = match sg0.segment with
+let rec append_seg_wf (#c : Type) (sg0 sg1 : cell_list c)
+  : Lemma (ensures wf_seg L.(sg0@sg1) <==>
+                   wf_seg sg0 /\ wf_seg sg1 /\ M.loc_disjoint (loc_seg sg0) (loc_seg sg1))
+          (decreases sg0)
+          [SMTPat (wf_seg L.(sg0@sg1))]
+  = match sg0 with
     | [] -> ()
-    | _ :: _ -> append_seg_wf (tail_seg sg0) sg1
+    | _ :: tl -> append_seg_wf tl sg1
 
-val append_seg_live (#a : Type) (h : HS.mem) (sg0 sg1 : list_seg a)
+val append_seg_live (#c : Type) (a : queue_param c) (h : HS.mem) (sg0 sg1 : list_seg c)
   : Lemma (requires sg0.exit == sg_entry sg1)
-          (ensures live_seg h (append_seg sg0 sg1) <==> live_seg h sg0 /\ live_seg h sg1)
+          (ensures live_seg a h (append_seg sg0 sg1) <==> live_seg a h sg0 /\ live_seg a h sg1)
           (decreases sg0.segment)
 
-val last_cell_live (#a : Type) (h : HS.mem) (sg : list_seg a)
-  : Lemma (requires live_seg h sg)
+val last_cell_live (#c : Type) (a : queue_param c) (h : HS.mem) (sg : list_seg c)
+  : Lemma (requires live_seg a h sg)
           (ensures B.live h (last_cell sg.segment))
           (decreases sg.segment)
 
 (** Segments handling *)
 
-noextract let empty_seg  (#a : Type) (exit : cell_ptr a) = { segment = []; exit }
-noextract let empty_list (a : Type) : list_nil a = empty_seg B.null
-val empty_live (#a : Type) (exit : B.pointer_or_null (cell a)) (h : HS.mem)
-  : Lemma (live_seg h (empty_seg #a exit)) [SMTPat (live_seg h (empty_seg #a exit))]
+noextract let empty_seg  (#c : Type) (exit : cell_ptr c) = { segment = []; exit }
+noextract let empty_list (c : Type) : list_nil c = empty_seg B.null
+val empty_live (#c : Type) (a : queue_param c) (exit : cell_ptr c) (h : HS.mem)
+  : Lemma (live_seg a h (empty_seg #c exit)) [SMTPat (live_seg a h (empty_seg #c exit))]
 
-let empty_sg_of_cell (#a : Type)
-  : Lemma (sg_of_cells #a [] == empty_list a) [SMTPat (sg_of_cells #a [])]
+let empty_sg_of_cell (#c : Type)
+  : Lemma (sg_of_cells #c [] == empty_list c) [SMTPat (sg_of_cells #c [])]
   = ()
 
-val sg_mkcons_lem (#a : Type) (h : HS.mem) (hd : B.pointer (cell a)) (tl : list_seg a)
+val sg_mkcons_lem (#c : Type) (a : queue_param c) (h : HS.mem) (hd : B.pointer c) (tl : list_seg c)
   : Lemma (requires B.live h hd /\
-                    g_cell_next h hd == sg_entry tl /\
-                    live_seg h tl)
-          (ensures  live_seg h (cons_seg hd tl))
+                    g_cell_next a h hd == sg_entry tl /\
+                    live_seg a h tl)
+          (ensures  live_seg a h (cons_seg hd tl))
 
-val sg_uncons_lem (#a : Type) (h : HS.mem) (sg : list_seg a)
-  : Lemma (requires live_seg h sg /\ Cons? sg.segment)
+val sg_uncons_lem (#c : Type) (a : queue_param c) (h : HS.mem) (sg : list_seg c)
+  : Lemma (requires live_seg a h sg /\ Cons? sg.segment)
           (ensures  (let cell = L.hd sg.segment in
                      let tl   = tail_seg sg     in
                      B.live h cell /\
-                     g_cell_next h cell == sg_entry tl /\
-                     live_seg h tl))
+                     g_cell_next a h cell == sg_entry tl /\
+                     live_seg a h tl))
 
 inline_for_extraction
-let sg_mkcons (#a : Type) (hd : G.erased (B.pointer (cell a))) (tl : G.erased (list_seg a))
-  : Stack (G.erased (list_seg a))
+let sg_mkcons (#c : Type) (a : queue_param c) (hd : G.erased (B.pointer c)) (tl : G.erased (list_seg c))
+  : Stack (G.erased (list_seg c))
           (requires fun h -> B.live h hd /\
-                          g_cell_next h hd == sg_entry tl /\
-                          live_seg h tl)
+                          g_cell_next a h hd == sg_entry tl /\
+                          live_seg a h tl)
           (ensures  fun h sg h' -> h' == h /\
                           G.reveal sg == cons_seg hd tl /\
-                          live_seg h sg)
-  = let h = ST.get () in sg_mkcons_lem h hd tl;
+                          live_seg a h sg)
+  = let h = ST.get () in sg_mkcons_lem a h hd tl;
     cons_seg hd tl
 
 inline_for_extraction
-let sg_mksglt (#a : Type) (hd : G.erased (B.pointer (cell a))) (exit : G.erased (cell_ptr a))
-  : Stack (G.erased (list_seg a))
+let sg_mksglt (#c : Type) (a : queue_param c) (hd : G.erased (B.pointer c)) (exit : G.erased (cell_ptr c))
+  : Stack (G.erased (list_seg c))
           (requires fun h -> B.live h hd /\
-                          g_cell_next h hd == G.reveal exit)
+                          g_cell_next a h hd == G.reveal exit)
           (ensures  fun h sg h' -> h' == h /\
                           G.reveal sg == { segment = [G.reveal hd]; exit } /\
-                          live_seg h sg)
-  = sg_mkcons hd (empty_seg exit)
+                          live_seg a h sg)
+  = sg_mkcons a hd (empty_seg exit)
 
 inline_for_extraction
-let sg_mkapp (#a : Type) (sg0 sg1 : G.erased (list_seg a))
-  : Stack (G.erased (list_seg a))
-          (requires fun h -> live_seg h sg0 /\ live_seg h sg1 /\
+let sg_mkapp (#c : Type) (a : queue_param c) (sg0 sg1 : G.erased (list_seg c))
+  : Stack (G.erased (list_seg c))
+          (requires fun h -> live_seg a h sg0 /\ live_seg a h sg1 /\
                           sg0.exit == sg_entry sg1)
           (ensures  fun h sg h' -> h' == h /\
                           G.reveal sg == append_seg sg0 sg1 /\
-                          live_seg h sg)
-  = let h = ST.get () in append_seg_live h sg0 sg1;
+                          live_seg a h sg)
+  = let h = ST.get () in append_seg_live a h sg0 sg1;
     append_seg sg0 sg1
 
 
 inline_for_extraction
-let sg_uncons (#a : Type) (sg : G.erased (list_seg a))
-  : Stack (G.erased (B.pointer (cell a)) & G.erased (list_seg a))
-          (requires fun h -> live_seg h sg /\ Cons? sg.segment)
+let sg_uncons (#c : Type) (a : queue_param c) (sg : G.erased (list_seg c))
+  : Stack (G.erased (B.pointer c) & G.erased (list_seg c))
+          (requires fun h -> live_seg a h sg /\ Cons? sg.segment)
           (ensures  fun h (cell, tl) h' -> h' == h /\
                      G.reveal sg == cons_seg cell tl /\
                      G.reveal tl == tail_seg sg /\
                      B.live h cell /\
-                     g_cell_next h cell == sg_entry tl /\
-                     live_seg h tl)
+                     g_cell_next a h cell == sg_entry tl /\
+                     live_seg a h tl)
   =
-    let h = ST.get () in sg_uncons_lem h sg;
+    let h = ST.get () in sg_uncons_lem a h sg;
     G.hide (L.hd sg.segment),
     G.hide (tail_seg sg)
 
 inline_for_extraction
-let sg_unapp (#a : Type) (sg0 sg1 : G.erased (list_seg a))
+let sg_unapp (#c : Type) (a : queue_param c) (sg0 sg1 : G.erased (list_seg c))
   : Stack  unit
-          (requires fun h -> live_seg h (append_seg sg0 sg1) /\
+          (requires fun h -> live_seg a h (append_seg sg0 sg1) /\
                           sg0.exit == sg_entry sg1)
           (ensures  fun h () h' -> h' == h /\
-                          live_seg h sg0 /\ live_seg h sg1)
-  = let h = ST.get () in append_seg_live h sg0 sg1
+                          live_seg a h sg0 /\ live_seg a h sg1)
+  = let h = ST.get () in append_seg_live a h sg0 sg1
 
-val entry_null_is_empty (#a : Type) (h : HS.mem) (sg : list_seg a)
-  : Lemma (requires live_seg h sg /\ B.g_is_null (sg_entry sg))
-          (ensures  sg == empty_list a)
-          [SMTPat (live_seg h sg)]
+val entry_null_is_empty (#c : Type) (a : queue_param c) (h : HS.mem) (sg : list_seg c)
+  : Lemma (requires live_seg a h sg /\ B.g_is_null (sg_entry sg))
+          (ensures  sg == empty_list c)
+          [SMTPat (live_seg a h sg)]
 
-val list_nil_entry_nnull (#a : Type) (h : HS.mem) (sg : list_nil a)
-  : Lemma (requires live_seg h sg /\ not (B.g_is_null (sg_entry sg)))
+val list_nil_entry_nnull (#c : Type) (a : queue_param c) (h : HS.mem) (sg : list_nil c)
+  : Lemma (requires live_seg a h sg /\ not (B.g_is_null (sg_entry sg)))
           (ensures  Cons? sg.segment)
-          [SMTPat (live_seg h sg); SMTPat (Cons? sg.segment)]
+          [SMTPat (live_seg a h sg); SMTPat (Cons? sg.segment)]
 
 inline_for_extraction
-val sgn_entry (#a : Type) (p : cell_ptr a) (sg : G.erased (list_nil a))
-  : Stack (cell_ptr a)
-                (requires fun h0       -> live_seg h0 sg /\ p == sg_entry sg)
+val sgn_entry (#c : Type) (a : queue_param c) (p : cell_ptr c) (sg : G.erased (list_nil c))
+  : Stack (cell_ptr c)
+                (requires fun h0       -> live_seg a h0 sg /\ p == sg_entry sg)
                 (ensures  fun h0 p' h1 -> h0 == h1 /\ B.live h1 p /\ p' == p)
 
 inline_for_extraction
-let sg_last (#a : Type) (p : cell_ptr a) (sg : G.erased (list_nil a))
-  : Stack (cell_ptr a)
-                (requires fun h0       -> live_seg h0 sg /\ p == last_cell sg.segment)
+let sg_last (#c : Type) (a : queue_param c) (p : cell_ptr c) (sg : G.erased (list_nil c))
+  : Stack (cell_ptr c)
+                (requires fun h0       -> live_seg a h0 sg /\ p == last_cell sg.segment)
                 (ensures  fun h0 p' h1 -> h0 == h1 /\ B.live h1 p /\ p' == p)
-  = let h = ST.get () in last_cell_live h sg;
+  = let h = ST.get () in last_cell_live a h sg;
     p
 
 inline_for_extraction
-val sg_next (#a : Type) (p : cell_ptr a) (sg : G.erased (list_seg a))
-  : Stack (cell_ptr a)
-          (requires fun h0       -> live_seg h0 sg /\ p == sg_entry sg /\ Cons? sg.segment)
+val sg_next (#c : Type) (a : queue_param c) (get_next : U.alias a.get_next)
+            (p : cell_ptr c) (sg : G.erased (list_seg c))
+  : Stack (cell_ptr c)
+          (requires fun h0       -> live_seg a h0 sg /\ p == sg_entry sg /\ Cons? sg.segment)
           (ensures  fun h0 p' h1 -> h0 == h1 /\
-                                 live_seg h1 (tail_seg sg) /\ p' == sg_entry (tail_seg sg))
+                                 live_seg a h1 (tail_seg sg) /\ p' == sg_entry (tail_seg sg))
 
 (** Lemmas *)
 
-let rec unsnoc_seg (#a : Type) (sg : list_seg a)
-  : Pure (list_seg a & list_seg a)
+let rec unsnoc_seg (#c : Type) (sg : list_seg c)
+  : Pure (list_seg c & list_seg c)
          (requires Cons? sg.segment)
          (ensures fun (ini, lt) ->
                    lt == { segment = [last_cell sg.segment]; exit = sg.exit } /\
@@ -318,7 +314,7 @@ let rec unsnoc_seg (#a : Type) (sg : list_seg a)
     | hd :: _ -> let ini, lt = unsnoc_seg (tail_seg sg) in
                cons_seg hd ini, lt
 
-let rec append_last_cell (#a : Type) (sg0 sg1 : list (B.pointer (cell a)))
+let rec append_last_cell (#c : Type) (sg0 sg1 : list (B.pointer c))
   : Lemma (requires  Cons? sg1)
           (ensures   last_cell L.(sg0@sg1) == last_cell sg1)
           (decreases sg0)
