Learn.LowStar.Queue.fst
@@ -1,5 +1,51 @@
 module Learn.LowStar.Queue
 
-include Learn.LowStar.Queue.Data
-include Learn.LowStar.Queue.Prop
-include Learn.LowStar.Queue.Impl
+module UL   = Learn.LowStar.Util
+module M    = LowStar.Modifies
+module Prop = Learn.LowStar.Queue.Prop
+module Impl = Learn.LowStar.Queue.Impl
+
+type queue c = Prop.queue c
+
+let loc_queue_st #c q =
+  M.loc_addr_of_buffer q
+let loc_queue #c q l =
+  M.(loc_union (loc_addr_of_buffer q) (Prop.loc_seg l))
+let wf_queue #c q l =
+  Prop.wf_seg l /\ M.(loc_disjoint (loc_addr_of_buffer q) (Prop.loc_seg l))
+let live_queue    = Prop.live_queue
+let freeable #c q = B.freeable q /\ True
+
+noextract inline_for_extraction let malloc   = Impl.malloc
+noextract inline_for_extraction let free     = Impl.free
+noextract inline_for_extraction let is_empty = Impl.is_empty
+
+noextract inline_for_extraction let enqueue #c a get_next set_next x q l =
+  Impl.enqueue #c a get_next set_next x q l;
+  let l' = L.snoc (G.reveal l,x) in
+  Prop.append_seg_wf l [x];
+  Prop.append_seg_loc l [x];
+  M.loc_union_assoc (M.loc_addr_of_buffer q) (Prop.loc_seg l) (Prop.loc_seg [x])
+
+noextract inline_for_extraction let dequeue #c a get_next q l =
+  let rt = Impl.dequeue #c a get_next q l in
+  UL.loc_union_comm12 (M.loc_addr_of_buffer q) (M.loc_buffer rt) (Prop.loc_seg (L.tl l));
+  rt
+
+noextract inline_for_extraction let find     = Impl.find
+
+
+let loc_queue_live_in #c a h q l =
+  Prop.loc_seg_live_in a h (Prop.sg_of_cells l)
+
+let frame_queue #c a h0 h1 q l r =
+  Prop.frame_seg #c a h0 h1 (Prop.sg_of_cells l) r
+
+let frame_queue_mod_data #c a h0 h1 q l r =
+  Prop.frame_seg_mod_data #c a h0 h1 (Prop.sg_of_cells l)
+
+let loc_queue_content #c q l x =
+  Prop.loc_seg_cell l x
+
+let live_queue_content #c a h q l x =
+  Prop.live_seg_cell a h (Prop.sg_of_cells l) x
