Learn.LowStar.Queue.Param.fst
@@ -1,0 +1,71 @@
+module Learn.LowStar.Queue.Param
+
+module Ll  = Learn.List
+module B   = LowStar.Buffer
+module M   = LowStar.Modifies
+module HS  = FStar.HyperStack
+
+(* [c] : type of cells *)
+
+type cell_ptr (c : Type) = B.pointer_or_null c
+
+type cell_list (c : Type) = list (B.pointer c)
+
+noeq type queue_param (c : Type) = {
+  get_next : c -> cell_ptr c;
+  set_next : c -> cell_ptr c -> c;
+  mod_next : c -> c -> prop;
+  get_set_next : (x : c) -> (y : cell_ptr c) ->
+                 Lemma (get_next (set_next x y) == y);
+  set_set_next : (x : c) -> (y0 : cell_ptr c) -> (y1 : cell_ptr c) ->
+                 Lemma (set_next (set_next x y0) y1 == set_next x y1);
+  mod_refl     : (x : c) ->
+                 Lemma (mod_next x x);
+  (* TODO? mod_trans *)
+  mod_set_next : (x : c) -> (y : cell_ptr c) ->
+                 Lemma (mod_next x (set_next x y))
+}
+
+
+let open_queue_param (#c : Type) (a : queue_param c)
+  : Lemma (ensures
+      (forall (x : c) (y : cell_ptr c) . {:pattern (a.get_next (a.set_next x y))}
+           a.get_next (a.set_next x y) == y) /\
+      (forall (x : c) (y0 y1 : cell_ptr c) . {:pattern (a.set_next (a.set_next x y0) y1)}
+           a.set_next (a.set_next x y0) y1 == a.set_next x y1) /\
+      (forall (x : c) . {:pattern (a.mod_next x x)}
+           a.mod_next x x) /\
+      (forall (x : c) (y : cell_ptr c) . {:pattern (a.mod_next x (a.set_next x y))}
+           a.mod_next x (a.set_next x y))
+    )
+  =
+    introduce forall (x : c) (y : cell_ptr c) . a.get_next (a.set_next x y) == y
+         with a.get_set_next x y;
+    introduce forall (x : c) (y0 y1 : cell_ptr c) . a.set_next (a.set_next x y0) y1 == a.set_next x y1
+         with a.set_set_next x y0 y1;
+    introduce forall (x : c) . a.mod_next x x
+         with a.mod_refl x;
+    introduce forall (x : c) (y : cell_ptr c) . a.mod_next x (a.set_next x y)
+         with a.mod_set_next x y
+
+
+let mod_next (#c : Type) (a : queue_param c) (h0 h1 : HS.mem) (x : B.pointer c) : GTot prop
+  = B.live h0 x /\ B.live h1 x /\ a.mod_next (B.deref h0 x) (B.deref h1 x)
+
+let mod_next_list (#c : Type) (a : queue_param c) (h0 h1 : HS.mem) (xs : cell_list c)
+  : GTot prop
+  = Ll.g_for_allP xs (mod_next a h0 h1)
+
+let mod_data (#c : Type) (a : queue_param c) (h0 h1 : HS.mem) (x : B.pointer c) : GTot prop
+  = B.live h0 x /\ B.live h1 x /\ a.get_next (B.deref h0 x) == a.get_next (B.deref h1 x)
+
+let mod_data_list (#c : Type) (a : queue_param c) (h0 h1 : HS.mem) (xs : cell_list c)
+  : GTot prop
+  = Ll.g_for_allP xs (mod_data a h0 h1)
+
+
+let disjoint_mod_next (#c : Type) (a : queue_param c) (h0 h1 : HS.mem) (p : M.loc) (x : B.pointer c)
+  : Lemma (requires M.(loc_disjoint (loc_buffer x) p /\ live h0 x /\ modifies p h0 h1))
+          (ensures  mod_next a h0 h1 x)
+          [SMTPat M.(modifies p h0 h1); SMTPat (mod_next a h0 h1 x)]
+  = a.mod_refl (B.deref h0 x)
