Learn.LowStar.Queue.Test.fst
@@ -1,0 +1,94 @@
+module Learn.LowStar.Queue.Test
+
+module Ll  = Learn.List
+module B   = LowStar.Buffer
+module M   = LowStar.Modifies
+module G   = FStar.Ghost
+module U32 = FStar.UInt32
+module HS  = FStar.HyperStack
+module ST  = FStar.HyperStack.ST
+
+open LowStar.BufferOps
+open FStar.HyperStack.ST
+
+open Learn.LowStar.Queue
+
+#push-options "--__no_positivity"
+noeq
+type cell = {
+  next: B.pointer_or_null cell;
+  data_x: U32.t;
+  data_y: bool
+}
+#pop-options
+
+noextract inline_for_extraction let get_next (x : cell) = x.next
+noextract inline_for_extraction let set_next (x : cell) (y : cell_ptr cell) = {x with next = y}
+
+noextract inline_for_extraction
+let a : queue_param cell = {
+  get_next = get_next;
+  set_next = set_next;
+  mod_next = (fun x x' -> x.data_x = x'.data_x /\ x.data_y = x'.data_y);
+  get_set_next = (fun _ _ -> ());
+  set_set_next = (fun _ _ _ -> ());
+  mod_refl     = (fun _ -> ());
+  mod_set_next = (fun _ _ -> ())
+}
+
+type queue = queue cell
+
+let malloc   = malloc   a
+let free     = free     a
+let is_empty = is_empty a
+let enqueue  = enqueue  a get_next set_next
+let dequeue  = dequeue  a get_next
+inline_for_extraction
+let find     = find     a get_next
+
+
+(* -------------------------------------------------------------- *)
+
+
+let mem_42 (q : queue) (l : G.erased (cell_list cell))
+  : Stack (cell_ptr cell)
+          (requires fun h       -> live_queue a h q l)
+          (ensures  fun h rt h' -> M.(modifies loc_none h h') /\
+                    rt == (match Ll.find_gtot (fun (c:B.pointer cell) -> (B.deref h c).data_x = 42ul) l with
+                           | Some p -> p | None -> B.null))
+  =   let h = ST.get () in
+    find q l h (fun c -> (B.deref h c).data_x = 42ul)
+               (fun c -> live_queue_content a h q l c; (c.(0ul)).data_x = 42ul)
+
+
+#push-options "--fuel 3 --z3rlimit 30"
+let test_queue_spec () : St unit
+  =
+    push_frame ();
+    let q = malloc HS.root in
+    let x0 = B.malloc #cell HS.root ({data_x = 5ul; data_y = true; next = B.null}) 1ul in
+    enqueue x0 q [];
+      (let h = ST.get () in assert (live_queue a h q [x0]));
+      (let d = (x0.(0ul)).data_x in assert (d == 5ul));
+      (let f = mem_42 q [x0] in assert (f == B.null));
+      (let h0 = ST.get () in
+    x0.(0ul) <- {x0.(0ul) with data_x = 42ul};
+      (let h1 = ST.get () in
+       frame_queue_mod_data a h0 h1 q [x0] (B.loc_buffer x0);
+       assert (live_queue a h1 q [x0])));
+      (let f = mem_42 q [x0] in assert (f == x0));
+
+    let x12 = B.alloca #cell ({data_x = 7ul; data_y = false; next = B.null}) 2ul in
+    let x1 = B.sub x12 0ul 1ul in let x2 = B.sub x12 1ul 1ul in
+    enqueue x1 q [x0];
+    x2.(0ul) <- {x2.(0ul) with data_y = true};
+    let x0' = dequeue q [x0; x1] in
+      assert (x0' == x0);
+    (*B.free x0; We only have that the queue is disjoint with [loc_buffer x0] but we cannot deduce
+                 that it is disjoint with [loc_addr_of_buffer x0] *)
+    let x1' = dequeue q [x1] in
+      (assert (x1' == x1); let d = (x1.(0ul)).data_x in assert (d = 7ul));
+    pop_frame ();
+    free q;
+    B.free x0
+#pop-options
