Learn.LowStar.Queue.fsti
@@ -1,0 +1,125 @@
+module Learn.LowStar.Queue
+
+include Learn.LowStar.Queue.Param
+
+module U   = Learn.Util
+module L   = FStar.List.Pure
+module Ll  = Learn.List
+module B   = LowStar.Buffer
+module M   = LowStar.Modifies
+module HS  = FStar.HyperStack
+module G   = FStar.Ghost
+open FStar.HyperStack.ST
+
+
+val queue (c : Type0) : Type0
+
+(* Ghost properties *)
+
+val loc_queue_st    (#c : Type) (q : queue c) : GTot M.loc
+
+val loc_queue       (#c : Type) (q : queue c) (l : cell_list c) : GTot M.loc
+
+val wf_queue        (#c : Type) (q : queue c) (l : cell_list c) : Tot prop
+
+val live_queue      (#c : Type) (a : queue_param c) (h : HS.mem) (q : queue c) (l : cell_list c) : Tot prop
+
+val freeable        (#c : Type) (q : queue c) : Tot prop
+
+(* Functions *)
+
+noextract inline_for_extraction
+val malloc (#c : Type) (a : queue_param c) (r : HS.rid)
+  : ST (queue c)
+       (requires fun _       -> is_eternal_region r)
+       (ensures  fun h0 q h1 -> M.(modifies loc_none h0 h1 /\
+                                fresh_loc (loc_queue_st q) h0 h1 /\
+                                loc_includes (loc_region_only true r) (loc_queue_st q)) /\
+                             freeable q /\
+                             wf_queue q [] /\ loc_queue q [] == loc_queue_st q /\ live_queue a h1 q [])
+
+noextract inline_for_extraction
+val free (#c : Type) (a : queue_param c) (q : queue c)
+  : ST  unit
+       (requires fun h      -> live_queue a h q [] /\ freeable q)
+       (ensures  fun h b h' -> M.(modifies (loc_queue_st q) h h'))
+
+noextract inline_for_extraction
+val is_empty (#c : Type) (a : queue_param c) (q : queue c) (l : G.erased (cell_list c))
+  : Stack  bool
+          (requires fun h      -> live_queue a h q l)
+          (ensures  fun h b h' -> h' == h /\ b = Nil? l)
+
+noextract inline_for_extraction
+val enqueue (#c : Type) (a : queue_param c) (get_next : U.alias a.get_next) (set_next : U.alias a.set_next)
+            (x : B.pointer c) (q : queue c) (l : G.erased (cell_list c))
+  : Stack  unit
+          (requires fun h0       -> wf_queue q l /\ live_queue a h0 q l /\
+                                 B.live h0 x /\
+                                 M.(loc_disjoint (loc_buffer x) (loc_queue q l)))
+          (ensures  fun h0 () h1 -> M.(modifies (loc_union (loc_queue q l) (loc_buffer x)) h0 h1) /\
+                                 mod_next a h0 h1 x /\ mod_next_list a h0 h1 l /\
+                                (let l' = L.snoc (G.reveal l,x) in
+                                 wf_queue q l' /\
+                                 live_queue a h1 q l' /\
+                                 M.(loc_queue q l' == loc_union (loc_queue q l) (loc_buffer x))))
+
+noextract inline_for_extraction
+val dequeue (#c : Type) (a : queue_param c) (get_next : U.alias a.get_next)
+            (q : queue c) (l : G.erased (cell_list c))
+  : Stack (B.pointer c)
+          (requires fun h0       -> wf_queue q l /\ live_queue a h0 q l /\
+                                 Cons? l)
+          (ensures  fun h0 rt h1 -> M.modifies (loc_queue q l) h0 h1 /\
+                                 mod_next_list a h0 h1 l /\
+                                 rt == L.hd l /\
+                                (let l' = L.tl l in
+                                 wf_queue q l' /\
+                                 live_queue a h1 q (L.tl l) /\ B.live h1 rt /\
+                                 M.(loc_queue q l == loc_union (loc_buffer rt) (loc_queue q l') /\
+                                    loc_disjoint (loc_buffer rt) (loc_queue q l'))))
+
+noextract inline_for_extraction
+val find (#c : Type) (a : queue_param c) (get_next : U.alias a.get_next)
+         (q : queue c) (l : G.erased (cell_list c))
+         (h0  : HS.mem)
+         (spec_f : (x : B.pointer c -> GTot bool))
+         (f : (x : B.pointer c) ->
+              Stack bool
+                    (requires fun h -> M.(modifies loc_none h0 h) /\ B.live h x /\ L.memP x l)
+                    (ensures  fun h b h' -> M.(modifies loc_none h h') /\ b = spec_f x))
+  : Stack (cell_ptr c)
+          (requires fun h       -> h == h0 /\ live_queue a h q l)
+          (ensures  fun h rt h' -> M.(modifies loc_none h h') /\
+                                rt == (match Ll.find_gtot spec_f l with
+                                       | Some p -> p | None -> B.null))
+
+(* Lemmas *)
+
+val loc_queue_live_in (#c : Type) (a : queue_param c) (h : HS.mem) (q : queue c) (l : cell_list c)
+  : Lemma (requires live_queue a h q l)
+          (ensures B.loc_in (loc_queue q l) h)
+    [SMTPat (live_queue a h q l)]
+
+val frame_queue (#c : Type) (a : queue_param c) (h0 h1 : HS.mem) (q : queue c) (l : cell_list c) (r : B.loc)
+  : Lemma (requires live_queue a h0 q l /\ M.(modifies r h0 h1 /\ loc_disjoint r (loc_queue q l)))
+          (ensures  live_queue a h1 q l)
+    [SMTPat (live_queue a h0 q l); SMTPat (M.modifies r h0 h1)]
+
+val frame_queue_mod_data (#c : Type) (a : queue_param c)
+                         (h0 h1 : HS.mem) (q : queue c) (l : cell_list c) (r : B.loc)
+  : Lemma (requires live_queue a h0 q l /\ M.(modifies r h0 h1 /\ loc_disjoint r (loc_queue_st q)) /\
+                    mod_data_list a h0 h1 l)
+          (ensures  live_queue a h1 q l)
+
+
+val loc_queue_content (#c : Type) (q : queue c) (l : cell_list c) (x : B.pointer c)
+  : Lemma (requires  L.memP x l)
+          (ensures   M.(loc_queue q l `loc_includes` loc_buffer x))
+
+val live_queue_content (#c : Type) (a : queue_param c)
+                       (h : HS.mem) (q : queue c) (l : cell_list c) (x : B.pointer c)
+  : Lemma (requires  live_queue a h q l /\ L.memP x l)
+          (ensures   B.live h x)
+
+(* TODO? : loc_queue q [] = loc_queue_st q, loc =, disjoint content ... *)
